lib/alloc, examples/cells: Add instances of Alloc typeclass

src/Rupicola/Lib/Alloc.v
@@ -30,6 +30,59 @@ Section with_parameters.
                         (Lift1Prop.ex1 (fun i => Lift1Prop.ex1 (P i px)))
     }.
 
+  (* FIXME if we need to roundtrip:
+
+     Class Allocable {A} (P : word.rep -> A -> mem -> Prop) :=
+       { alloc_sz: Z;
+         alloc_length_ok bs := Z.of_nat (List.length bs) = alloc_sz;
+         alloc_sz_ok : alloc_sz mod Memory.bytes_per_word width = 0;
+
+         alloc_to_bytes : A -> list byte;
+         alloc_of_bytes : forall bs: list byte, alloc_length_ok bs -> A;
+
+         alloc_to_bytes_length_ok a: alloc_length_ok (alloc_to_bytes a);
+
+         alloc_to_bytes_ok ptr bs:
+           Lift1Prop.impl1
+             (P ptr bs)
+             (array ptsto (word.of_Z 1) ptr (alloc_to_bytes bs));
+         alloc_of_bytes_ok ptr bs (Hlen: alloc_length_ok bs) :
+           Lift1Prop.impl1
+             (array ptsto (word.of_Z 1) ptr bs)
+             (P ptr (alloc_of_bytes bs Hlen)) }.
+
+     Lemma alloc_of_bytes_to_bytes
+           {A} (P : word.rep -> A -> mem -> Prop)
+           `{Allocable _ P} a Hlen:
+       alloc_of_bytes (alloc_to_bytes a) Hlen = a.
+     Proof. … Qed. *)
+
+  Class SimpleAllocable {A} (P : word.rep -> A -> mem -> Prop) :=
+    { ssize_in_bytes : Z;
+      ssize_in_bytes_mod :
+        ssize_in_bytes mod Memory.bytes_per_word width = 0;
+      sP_to_bytes px x :
+        Lift1Prop.impl1 (P px x) (Memory.anybytes px ssize_in_bytes);
+      sP_from_bytes px :
+        Lift1Prop.impl1 (Memory.anybytes px ssize_in_bytes)
+                        (Lift1Prop.ex1 (P px)) }.
+
+  Instance Allocable_of_SimpleAllocable {A} (P : word.rep -> A -> mem -> Prop)
+           {H: SimpleAllocable P} : Allocable (fun _: unit => P).
+  Proof.
+    refine {| size_in_bytes := ssize_in_bytes;
+              size_in_bytes_mod := ssize_in_bytes_mod;
+              P_to_bytes := _;
+              P_from_bytes := _ |}; intros.
+    - apply sP_to_bytes.
+    - abstract (red; exists tt; apply sP_from_bytes; assumption).
+  Defined.
+
+  Program Instance SimpleAllocable_scalar : SimpleAllocable scalar :=
+    {| ssize_in_bytes := Memory.bytes_per_word width;
+       ssize_in_bytes_mod := Z_mod_same_full _;
+       sP_to_bytes := scalar_to_anybytes;
+       sP_from_bytes := anybytes_to_scalar |}.
 
   Definition pred_sep {A} R (pred : A -> predicate) (v : A) tr' mem' locals':=
     (R * (fun mem => pred v tr' mem locals'))%sep mem'.
@@ -38,6 +91,7 @@ Section with_parameters.
   (*TODO: should this require finding the instance? probably not
    Definition alloc {p : Semantics.parameters} {A} {P : A -> @Semantics.mem p -> Prop} `{@Allocable p A P} (a : A) := a. *)
   Definition alloc {A} (a : A) := a. 
+  Definition simple_alloc {A} (a : A) := a.
 
   Lemma compile_alloc
         {tr m l functions A} (v : A):
@@ -91,11 +145,36 @@ Section with_parameters.
       apply map.split_comm; eauto.
     }
   Qed.
-  
+
+  Lemma compile_simple_alloc {tr m l functions A} (v : A):
+    forall {P} {pred: P v -> predicate} {k: nlet_eq_k P v} {k_impl}
+      {AP : word.rep -> A -> map.rep -> Prop} `{SimpleAllocable A AP}
+      (R: mem -> Prop) out_var,
+
+      R m ->
+
+      (forall out_ptr uninit m',
+          sep (AP out_ptr uninit) R m' ->
+          <{ Trace := tr;
+             Memory := m';
+             Locals := map.put l out_var out_ptr;
+             Functions := functions }>
+          k_impl
+          <{ pred_sep (Memory.anybytes out_ptr size_in_bytes)
+                      pred (nlet_eq [out_var] v k) }>) ->
+      <{ Trace := tr;
+         Memory := m;
+         Locals := l;
+         Functions := functions }>
+      cmd.stackalloc out_var size_in_bytes k_impl
+      <{ pred (nlet_eq [out_var] (simple_alloc v) k) }>.
+  Proof.
+    intros; eapply compile_alloc; eauto.
+  Qed.
 End with_parameters.
 
-
 Arguments alloc : simpl never.
+Arguments simple_alloc : simpl never.
 Arguments size_in_bytes : simpl never.
 
 (*TODO: speed up by combining pred_seps first and using 1 proper/ecancel_assumption?*)
@@ -111,5 +190,7 @@ Ltac clear_pred_seps :=
 (* FIXME I don't think eassumption is needed, and there might actually be multiple ?R m *)
 #[export] Hint Extern 10 =>
   simple eapply compile_alloc; [eassumption | shelve] : compiler.
+#[export] Hint Extern 10 =>
+  simple eapply compile_simple_alloc; shelve : compiler.
 #[export] Hint Extern 1 (pred_sep _ _ _ _ _ _) =>
   clear_pred_seps; shelve : compiler_cleanup_post.
